lean/LoVe/LoVe02_ProgramsAndTheorems_HomeworkSheet.lean
@@ -23,14 +23,16 @@ namespace LoVe
 list. Your function should be defined by recursion and not using `++`
 (`List.append`). -/
 
-def snoc {α : Type} : List α → α → List α :=
-  sorry
+def snoc {α : Type} : List α → α → List α
+  | [], a => [a]
+  | (x :: xs), a => x :: snoc xs a
 
 /- 1.2. Convince yourself that your definition of `snoc` works by testing it on
 a few examples. -/
 
 #eval snoc [1] 2
 -- invoke `#eval` or `#reduce` here
+#eval snoc [1, 2, 3] 4
 
 
 /- ## Question 2: Minus 2
@@ -39,14 +41,19 @@ a few examples. -/
 
 Hint: There should be three cases. -/
 
-def minusTwo : ℕ → ℕ :=
-  sorry
+def minusTwo : ℕ → ℕ
+  | 0 => 0
+  | 1 => 0
+  | Nat.succ (Nat.succ n) => n
 
 /- 2.2. Convince yourself that your definition of `minusTwo` works by testing
 it on a few examples. -/
 
 #eval minusTwo 0   -- expected: 0
 -- invoke `#eval` or `#reduce` here
+#eval minusTwo 1
+#eval minusTwo 2
+#eval minusTwo 5
 
 
 /- ## Question 3: Sum
@@ -54,8 +61,9 @@ it on a few examples. -/
 3.1. Define a `sum` function that computes the sum of all the numbers in a
 list. -/
 
-def sum : List ℕ → ℕ :=
-  sorry
+def sum : List ℕ → ℕ
+  | [] => 0
+  | x :: xs => x + sum xs
 
 #eval sum [1, 12, 3]   -- expected: 16
 
@@ -108,5 +116,9 @@ Hint: Take a look at `reverse_reverse` from the demonstration file. -/
 #check SorryTheorems.reverse_reverse
 
 -- enter your theorem statements here
+
+theorem append_assoc {α : Type} (xs : List α) (ys : List α) (zs : List α) :
+    append _ (append _ xs ys) zs = append _ xs (append _ ys zs) :=
+  sorry
 
 end LoVe
